FokkerChallenge/TwoVarsAreNotEnough/Subterms.lean
@@ -1,35 +1,35 @@
 import FokkerChallenge.TwoVarsAreNotEnough.Basic
+import FokkerChallenge.EnhancedCslib.Closedunderapp
+import FokkerChallenge.EnhancedCslib.GenFinset
 
 namespace Cslib
 
 namespace LambdaCalculus.LocallyNameless.Untyped.Term
 
-@[scoped grind =]
-def subterms : Term String -> Finset (Term String)
+@[simp, scoped grind =]
+def subterms : Term String -> List (Term String)
   | Term.bvar _ => ∅
   | Term.fvar _ => ∅
-  | Term.abs (Term.abs t) => insert t.abs.abs (subterms t)
+  | Term.abs (Term.abs t) => t.abs.abs :: (subterms t)
   | Term.abs _ => ∅
   | Term.app t1 t2 => subterms t1 ∪ subterms t2
 
 theorem subterms_subset {t : Term String} :
     ∀ s ∈ t.subterms, s.subterms ⊆ t.subterms := by
   induction h : t.fokker_size using Nat.strong_induction_on generalizing t with
-  | h n _ => cases t with
-  | bvar _ => grind
-  | fvar _ => grind
+  | h n _ => cases t with (simp_all; try subst_vars)
   | app _ _ => grind
-  | abs t => cases t with grind
+  | abs t => cases t with (simp_all; try subst_vars)
+    | abs _ => grind
 
 @[scoped grind]
 theorem subterms_size {t} :
     ∀ s ∈ subterms t, s.fokker_size <= t.fokker_size := by
   induction h : t.fokker_size using Nat.strong_induction_on generalizing t with
-  | h n _ => cases t with
-  | bvar _ => grind
-  | fvar _ => grind
+  | h n _ => cases t with (simp_all; try subst_vars)
   | app _ _ => grind
-  | abs t => cases t with grind
+  | abs t => cases t with (simp_all; try subst_vars)
+    | abs _ => grind
 
 /-
 theorem subterms_gen {t M} (h : Gen t M) : t.subterms = M.subterms := by
@@ -39,11 +39,10 @@ theorem subterms_gen {t M} (h : Gen t M) : t.subterms = M.subterms := by
 theorem subterms_fv {t} (h : t.fv = ∅) :
     ∀ s ∈ subterms t, s.fv = ∅ := by
     induction h : t.fokker_size using Nat.strong_induction_on generalizing t with
-    | h n _ => cases t with
-      | bvar _ => grind
-      | fvar _ => grind
+    | h n _ => cases t with  (simp_all; try subst_vars)
       | app _ _ => grind
-      | abs t => cases t with grind
+      | abs t => cases t with (simp_all; try subst_vars)
+        | abs _ => grind
 
 theorem subterms_preserved_under_openRec {x i t} (h : two_vars_are_enough t) :
     t.subterms = t⟦i ↝ fvar x⟧.subterms := by
@@ -58,15 +57,36 @@ theorem subterms_preserved_under_openRec {x i t} (h : two_vars_are_enough t) :
 theorem subterms_two_vars_are_enough {t} (h : two_vars_are_enough t) :
     ∀ s ∈ subterms t, abs_two_vars_are_enough s := by
     induction h : t.fokker_size using Nat.strong_induction_on generalizing t with
-    | h n _ => cases t with
-      | bvar _ => grind
-      | fvar _ => grind
+    | h n _ => cases t with (simp_all; try subst_vars)
       | app _ _ => grind
-      | abs t => cases t with grind
+      | abs t => cases t with (simp_all; try subst_vars)
+        | abs _ => grind
 
 theorem two_vars_are_enough_subterms_lc {t} (h : two_vars_are_enough t) :
     ∀ s ∈ subterms t, s.LC := by grind
 
+theorem subterms_closedunderappbool {t} (h : ClosedUnderAppBool abs_two_vars_are_enough t) :
+    ∀ s ∈ subterms t, abs_two_vars_are_enough s := by
+    induction h : t.fokker_size using Nat.strong_induction_on generalizing t with
+    | h n _ => cases t with (simp_all; try subst_vars)
+      | app _ _ => grind
+      | abs t => cases t with (simp_all; try subst_vars)
+        | abs _ => grind
+
+theorem closedUnderAppBool_genfinset_subterms {t} (h : ClosedUnderAppBool abs_two_vars_are_enough t) :
+    GenFinset t.subterms t := by
+    induction ht : t.fokker_size using Nat.strong_induction_on generalizing t with | h n ih =>
+    cases t with
+    | bvar _ => cases h
+    | fvar _ => cases h
+    | abs t => cases t <;> grind
+    | app x y =>  have := @ih x.fokker_size (by grind) x (by grind) rfl
+                  have := @ih y.fokker_size (by grind) y (by grind) rfl
+                  refine .app ?_ ?_
+                  . grind [genfinset_concat_l, genfinset_concat_r]
+                  . grind [genfinset_concat_l, genfinset_concat_r]
+
+/-
 @[scoped grind =]
 def idempotent (terms : Finset (Term String)) : Prop :=
   terms.biUnion subterms = terms
@@ -78,3 +98,4 @@ theorem subterms_idempotent {t : Term String} : idempotent t.subterms := by
     | fvar _ => grind
     | app _ _ => grind
     | abs t => cases t with grind
+-/
