FokkerChallenge/EnhancedCslib/GenFinset.lean
@@ -8,13 +8,17 @@ namespace Cslib
 
 namespace LambdaCalculus.LocallyNameless.Untyped.Term
 
+@[simp, scoped grind unfold]
 def GenFinset (atoms: List (Term String)) := ClosedUnderApp (fun t => t ∈ atoms)
 
+@[simp, scoped grind unfold]
 def Gen (atom : Term String) := GenFinset [atom]
 
+@[simp, scoped grind unfold]
 def not_basises (atoms : List (Term String)) : Prop :=
   ∃ y, y.LC ∧ y.fv = ∅ ∧ ∀ t, GenFinset atoms t → Relation.ReflTransGen FullBetaEta t y → False
 
+@[simp, scoped grind unfold]
 def not_basis (atom : Term String) : Prop := not_basises [atom]
 
 theorem genfinset_depth {fs M} (h : GenFinset fs M) :
@@ -25,3 +29,11 @@ theorem genfinset_depth {fs M} (h : GenFinset fs M) :
                   List.mem_le_max?_getD (List.mem_map_of_mem ht)
                 omega
   | app _ _ _ _ => unfold depth; omega
+
+theorem genfinset_concat_l {l1 l2 M} (h : GenFinset l1 M) :
+  GenFinset (l1 ∪ l2) M := by
+  induction h <;> grind
+
+theorem genfinset_concat_r {l1 l2 M} (h : GenFinset l2 M) :
+  GenFinset (l1 ∪ l2) M := by
+  induction h <;> grind
